Bump Iris
Changes are for discardable fractions in saved props
(https://gitlab.mpi-sws.org/iris/iris/-/merge_requests/802).

src/base_logic/lib/saved_spec.v
@@ -13,7 +13,7 @@ Notation savedSpecΣ In Out := (savedAnythingΣ (In -d> (Out -d> ▶ ∙) -n> �
 Program Definition saved_spec_own {In Out : Type} `{!savedSpecG Σ In Out} (γ : gname)
     (Spec : savedSpecO Σ In Out)
   :=
-  saved_anything_own (F := In -d> (Out -d> ▶ ∙) -n> ▶ ∙) γ
+  saved_anything_own (F := In -d> (Out -d> ▶ ∙) -n> ▶ ∙) γ dfrac.DfracDiscarded
     (λ in_, (λne Φ : Out -d> laterO (iPropO Σ), Next (Spec in_ (λ out, later_car (Φ out))))).
 Next Obligation.
   intros ????? Spec ?? Φ1 Φ2 HΦ.
@@ -42,11 +42,19 @@ Proof. iIntros (?). rewrite /saved_spec_own. by iApply saved_anything_alloc_stro
 
 Lemma saved_spec_alloc_cofinite (G : gset gname) Spec :
   ⊢ |==> ∃ γ, ⌜γ ∉ G⌝ ∗ saved_spec_own γ Spec.
-Proof. rewrite /saved_spec_own. iApply saved_anything_alloc_cofinite. Qed.
+Proof.
+  rewrite /saved_spec_own.
+  iApply saved_anything_alloc_cofinite.
+  apply (dfrac.dfrac_valid_discarded 1).
+Qed.
 
 Lemma saved_spec_alloc Spec :
   ⊢ |==> ∃ γ, saved_spec_own γ Spec.
-Proof. rewrite /saved_spec_own. iApply saved_anything_alloc. Qed.
+Proof.
+  rewrite /saved_spec_own.
+  iApply saved_anything_alloc.
+  apply (dfrac.dfrac_valid_discarded 1).
+Qed.
 
 (* We put the `x` on the outside to make this lemma easier to apply. *)
 Lemma saved_spec_agree γ Spec1 Spec2 x Φ :
