src/program_logic/staged_invariant_use_cancel.v
@@ -26,10 +26,10 @@ Definition staged_value_inuse_cancel e E1' E1 mj mj_wp mj_ukeep Φ Φc P :=
       ⌜ (mj_wp ≤ / 2 + mj_ishare) ⌝%Qp ∗
       own γsaved (◯ Excl' (γprop, γprop')) ∗
       own γstatus (◯ Excl' (inuse mj_wp mj_ushare)) ∗
-      saved_prop_own γprop (wpc0 NotStuck mj_wp E1 e
+      saved_prop_own γprop DfracDiscarded (wpc0 NotStuck mj_wp E1 e
                      (λ v : val Λ, staged_inv_cancel E1 mj_wp P ∗ (Φc ∧ Φ v))
                      (Φc ∗ P)) ∗
-      saved_prop_own γprop' Φc ∗
+      saved_prop_own γprop' DfracDiscarded Φc ∗
       later_tok ∗
       pri_inv_tok mj_ukeep E2 ∗
       ⌜ /2 < mj ⌝%Qp ∗
@@ -82,6 +82,7 @@ Proof.
     {
       iDestruct "Hfin" as "(HPR&Hrest)".
       iMod (saved_prop_alloc True%I) as (γprop_remainder') "#Hsaved2''".
+      { apply (dfrac_valid_discarded 1). }
       iMod (own_update_2 _ _ _ (● Excl' (γprop_stored, γprop_remainder') ⋅
                                   ◯ Excl' (γprop_stored, γprop_remainder'))
               with "Hown' Hown") as "[Hown' Hown]".
@@ -121,6 +122,7 @@ Proof.
     rewrite -Heq_mj.
     iDestruct (pri_inv_tok_split with "Hitok") as "(Hitok_ukeep&Hitok_ushare)".
     iMod (saved_prop_alloc True%I) as (γprop_remainder') "#Hsaved2''".
+    { apply (dfrac_valid_discarded 1). }
     iMod (own_update_2 _ _ _ (● Excl' (γprop_stored, γprop_remainder') ⋅
                                 ◯ Excl' (γprop_stored, γprop_remainder'))
             with "Hown' Hown") as "[Hown' Hown]".
@@ -231,7 +233,9 @@ Proof.
     iMod (saved_prop_alloc
             (wpc0 NotStuck mj_wp ⊤ e2 (λ v : val Λ, staged_inv_cancel _ mj_wp P ∗ Φc ∧ Φ v)
               (Φc ∗ P))%I) as (γprop_stored') "#Hsaved1''".
+    { apply (dfrac_valid_discarded 1). }
     iMod (saved_prop_alloc Φc) as (γprop_remainder') "#Hsaved2''".
+    { apply (dfrac_valid_discarded 1). }
     iMod (own_update_2 _ _ _ (● Excl' (γprop_stored', γprop_remainder') ⋅
                               ◯ Excl' (γprop_stored', γprop_remainder'))
             with "Hown' Hown") as "[Hown' Hown]".
@@ -434,7 +438,9 @@ Proof.
     iMod (saved_prop_alloc
             (wpc0 NotStuck mj_wp ⊤ e2 (λ v : val Λ, staged_inv_cancel ⊤ mj_wp P ∗ Φc ∧ Φ v)
               (Φc ∗ P))%I) as (γprop_stored') "#Hsaved1''".
+    { apply (dfrac_valid_discarded 1). }
   iMod (saved_prop_alloc Φc) as (γprop_remainder') "#Hsaved2''".
+  { apply (dfrac_valid_discarded 1). }
   iMod (own_update_2 _ _ _ (● Excl' (γprop_stored', γprop_remainder') ⋅
                             ◯ Excl' (γprop_stored', γprop_remainder'))
           with "Hown' Hown") as "[Hown' Hown]".
